\batchmode
\documentclass{article}
\usepackage{epsfig}
\usepackage{amsmath}
\usepackage{amssymb}
\usepackage{amsthm}
\pagestyle{empty}
\begin{document}
\[ \Omega=[0,1]^d\ \subset\ \mathbb{R}^d \]
\pagebreak

\[ \Omega=\{ \mathbf{x} \in \mathbb{R}^d | x_i \geq 0, \sum_{i=1}{d} x_i \leq 1 \} \]
\pagebreak

$ d=1,2,3 $
\pagebreak

$ \mathbf{x}=(x_1,...,x_d) $
\pagebreak

$ \int_\Omega 1 $
\pagebreak

$ \int_{\partial\Omega} 1 $
\pagebreak

$ \int_{\Omega} x^2+y^2+z^2 $
\pagebreak

$ (x,y,z) \mapsto x^2+y^2+z^2$
\pagebreak

$y=z=0$
\pagebreak

$ z=0 $
\pagebreak

$ \int_{\Omega} sin(x^2+y^2+z^2) $
\pagebreak

$ (x,y,z) \mapsto sin(x^2+y^2+z^2)$
\pagebreak

$ X_h $
\pagebreak

$ X_h$
\pagebreak

\begin{eqnarray} g(x,y,z) &=& \sin(\pi x/2)\ \cos(\pi y/2)\ \cos(\pi*z/2) \\ f(x,y,z) &=& (1-x^2)\ (1-y^2)\ (1-z^2)\ (x^2+y^2+z^2)^{\alpha/2.0},\quad \alpha=3 \end{eqnarray}
\pagebreak

\[ -\Delta u = f\ \text{in}\ \Omega = [-1;1]^2 \]
\pagebreak

\[ f= 2 \pi^2 g \]
\pagebreak

\[ g=\sin(\pi x) \cos(\pi y) \]
\pagebreak

\[ u=g_{|x=\pm 1}, \quad \frac{\partial u}{\partial n} = 0_{|y=\pm 1} \]
\pagebreak

\[ \mathcal{X} = \Big\{ v \in H_1(\Omega) \text{ such that } v=g_{|x=-1,x=1} \Big\} \]
\pagebreak

\[ \mathcal{V} = \Big\{ v \in H_1(\Omega) \text{ such that } v=0_{|x=-1,x=1} \Big\} \]
\pagebreak

$v \in \mathcal{V}$
\pagebreak

\begin{equation} \label{eq:13} \int_\Omega -\Delta u v = \int_\Omega f v \end{equation}
\pagebreak

$u \in \mathcal{X}$
\pagebreak

\[ \int_\Omega \nabla u \cdot \nabla v = \int_\Omega f v \]
\pagebreak

\[ \int_{\partial \Omega} \frac{\partial u}{\partial n} v = 0, \]
\pagebreak

\[ \label{eq:21} \frac{\partial u}{\partial n} \stackrel{\text{def}}{=} \nabla u \cdot n \]
\pagebreak

$\partial \Omega$
\pagebreak

\[ \label{eq:10} \Omega = \cup_{e=1}^\nel \Omega^e \]
\pagebreak

$d$
\pagebreak

$\nel$
\pagebreak

$N$
\pagebreak

\[ \label{eq:17} X_h = \Big\{ v_h \in C^0(\Omega),\ {v_h}_{|\Omega^e} \in \mathbb{P}_N( \Omega^e ),\ v_h=g_{|x=-1,x=1}\Big\} \]
\pagebreak

\[ \label{eq:18} V_h = \Big\{ v_h \in C^0(\Omega),\ {v_h}_{|\Omega^e} \in \mathbb{P}_N( \Omega^e ),\ v_h=0_{|x=-1,x=1}\Big\} \]
\pagebreak

$u_h \in X_h \subset \mathcal{X}$
\pagebreak

$v \in V_h \subset \mathcal{V}$
\pagebreak

\[ \int_\Omega \nabla u_h \cdot \nabla v_h = \int_\Omega f v_h \]
\pagebreak

$u \in X_h \subset H_1(\Omega)$
\pagebreak

$v \in X_h$
\pagebreak

\[ \int_\Omega \nabla u \cdot \nabla v + \int_{|x=-1,x=1} -\frac{\partial u}{\partial n} v - u \frac{\partial v}{\partial n} + \frac{\mu}{h} u v = \int_\Omega f v + \int_{|x=-1,x=1} - g \frac{\partial v}{\partial n} + \frac{\mu}{h} g v \]
\pagebreak

\[ \label{eq:19} X_h = \Big\{ v_h \in C^0(\Omega),\ {v_h}_{|\Omega^e} \in \mathbb{P}_N( \Omega^e ) \Big\} \]
\pagebreak

$> 0$
\pagebreak

$h$
\pagebreak

\[ \begin{array}{rccl} \ell: & X_h & \mapsto & \mathbb{R}\\ & v_h & \rightarrow &\ell(v_h)=\int_\Omega f v_h \end{array} \]
\pagebreak

$x=\pm 1$
\pagebreak

$1$
\pagebreak

$3$
\pagebreak

$x=-1$
\pagebreak

$x=1$
\pagebreak

\[ D u = F \]
\pagebreak

$L_2$
\pagebreak

\begin{equation} \label{eq:7} \|u-u_h\|_{L_2}\ =\ \sqrt{\int_\Omega (u-u_h)^2} = \sqrt{\int_\Omega (g-u_h)^2} \end{equation}
\pagebreak

$u_h$
\pagebreak

$h^{-(N+1)}$
\pagebreak

$h^{-N}$
\pagebreak

$(\mathbf{u},p)$
\pagebreak

$p$
\pagebreak

$p+c$
\pagebreak

\[ \label{eq:26} \int_\Omega p = 0 \]
\pagebreak

$(\mathbf{u},p,\lambda)$
\pagebreak

\[ - \mu \Delta \mathbf{u} +\nabla p = \mathbf{f}\quad, \quad \nabla \cdot \mathbf{u} + \lambda = 0, \quad \text{and}\quad \int_\Omega p = 0,\quad \text{in}\ \Omega = [-1;1]^2 \]
\pagebreak

\[ \mathbf{f} = \mathbf{0} \]
\pagebreak

\[ \mathbf{u}=\mathbf{1}_{|y=1}, \quad \mathbf{u}=\mathbf{0}_{|\partial \Omega \backslash \{(x,y) \in \Omega | y=1\}} \]
\pagebreak

$\mathbf{u}$
\pagebreak

$H^1_0(\Omega)$
\pagebreak

$L^2_0(\Omega)$
\pagebreak

$L^2(\Omega)$
\pagebreak

$\mathbb{P}_0(\Omega)$
\pagebreak

$\mathcal{X} = H^1_0(\Omega)\times L^2(\Omega)\times\mathbb{P}_0(\Omega)$
\pagebreak

$(\mathbf{u}, p, \lambda) \in \mathcal{X}$
\pagebreak

$(\mathbf{v},q,\nu) \in \mathcal{X}$
\pagebreak

\[ \int_\Omega \mu \nabla \mathbf{u} : \nabla \mathbf{v} + \nabla \cdot \mathbf{v} p + \nabla \cdot \mathbf{u}\ q + q \lambda + p \nu \ = \ \int_\Omega \mathbf{f} \cdot \mathbf{v} \]
\pagebreak

$\Omega_h$
\pagebreak

$M_h$
\pagebreak

$\mathbb{P}_N/\mathbb{P}_{N-1}$
\pagebreak

$\mathcal{X}_h=X_h\times M_h \times \mathbb{P}_0(\Omega)$
\pagebreak

$(\mathbf{u}_h,p_h,\lambda_h) \in \mathcal{X}_h$
\pagebreak

$(\mathbf{v}_h,q_h,\nu_h) \in \mathcal{X}_h$
\pagebreak

\[ \label{eq:27} \int_{\Omega_h} \mu \nabla \mathbf{u}_h \cdot \nabla \mathbf{v}_h + \nabla \cdot \mathbf{v}_h \ p_h + \nabla \cdot \mathbf{u}_h\ q_h + p_h \nu_h + q_h \lambda_h = \ \int_{\Omega_h} \mathbf{f} \cdot \mathbf{v}_h \]
\pagebreak

\[ \label{eq:28} \underbrace{\begin{pmatrix} A & B & 0\\ B^T & 0 & C\\ 0 & C^T & 0 \end{pmatrix}}_{\mathcal{A}} \underbrace{ \begin{pmatrix} \mathbf{u}_h\\ p_h\\ \lambda_h \end{pmatrix}}_{\mathcal{U}} = \underbrace{\begin{pmatrix} F\\ 0\\ 0 \end{pmatrix}}_{\mathcal{F}} \]
\pagebreak

$(\mathbf{u},\mathbf{v})$
\pagebreak

$(\mathbf{u},q)$
\pagebreak

$C$
\pagebreak

$(p,\nu)$
\pagebreak

$\mathcal{A}$
\pagebreak

$\mathcal{A} \mathcal{U} = \mathcal{F}$
\pagebreak

$\mathcal{X}_h$
\pagebreak

$\mathcal{U}$
\pagebreak

$\mathcal{F}$
\pagebreak

$\lambda$
\pagebreak

$\mathbb{P}_0(\Omega_h)$
\pagebreak

$\tau(\mathbf{u}) = \frac{1}{2}(\nabla \mathbf{u} + \nabla \mathbf{u}^T)$
\pagebreak

$\tau(\mathbf{u}) = \nabla \mathbf{u}$
\pagebreak

$\bar{\sigma}(\mathbf{u},p) \mathbf{n} = -p \mathbf{n} + 2 \mu \tau(\mathbf{u}) \mathbf{n}$
\pagebreak

$\mathbf{n}$
\pagebreak

$\bar{\sigma}(\mathbf{u},p) = -p \mathbb{I} + 2 \mu \tau(\mathbf{u})$
\pagebreak

\end{document}
